bedrock2/src/TailRecursion.v
@@ -4,15 +4,106 @@ From bedrock2 Require Import WeakestPrecondition WeakestPreconditionProperties.
 From bedrock2 Require Import Map Map.Separation Map.SeparationLogic.
 
 Section TailRecrsion.
-  Context {p : unique! Semantics.parameters}.
-  Local Infix "*" := Separation.sep.
-  Local Infix "*" := Separation.sep : type_scope.
-  Local Infix "==>" := Lift1Prop.impl1.
-  Lemma tailrecursion {mem_ok:Map.map.ok mem} {rely guarantee progress call}
+  Context
+    {p : unique! Semantics.parameters}
+    {rely guarantee : trace -> Prop}
+    {progress : trace -> trace -> Prop}
+    {call : funname -> trace -> mem -> list word -> (trace -> mem -> list word -> Prop) -> Prop}
     {Proper_call : Proper (pointwise_relation _ (pointwise_relation _
       (pointwise_relation _ (pointwise_relation _ (pointwise_relation _
       (pointwise_relation _ (pointwise_relation _ Basics.impl)) ==>
-      Basics.impl)))))%signature call}
+      Basics.impl)))))%signature call}.
+
+  Lemma tailrec
+    e c t (m : mem) l (post : _->_->_-> Prop)
+    {measure : Type} (P Q:_->_->_->_->Prop) lt (Hwf : well_founded lt) (v0 : measure)
+    (Hpre : P v0 t m l)
+    (Hbody : forall v t m l, P v t m l ->
+      exists br, expr m l e (eq br) /\
+      (word_test br = true -> cmd rely guarantee progress call c t m l
+        (fun t' m' l' => exists v', P v' t' m' l' /\
+          (progress t' t \/ lt v' v) /\
+          forall T M L, Q v' T M L -> Q v T M L)) /\
+      (word_test br = false -> Q v t m l))
+    (Hpost : forall t m l, Q v0 t m l -> post t m l)
+    : cmd rely guarantee progress call (cmd.while e c) t m l post.
+  Proof.
+    eexists measure, lt, (fun v t m l => P v t m l /\
+                          forall T M L, Q v T M L -> Q v0 T M L).
+    split. assumption.
+    split; [solve[eauto]|].
+    intros vi ti mi li (?&Qi).
+    destruct (Hbody _ _ _ _ ltac:(eassumption)) as (br&?&X); exists br; split; [assumption|].
+    destruct X as (Htrue&Hfalse). split; intros Hbr;
+      [pose proof(Htrue Hbr)as Hpc|pose proof(Hfalse Hbr)as Hpc]; clear Hbr Htrue Hfalse.
+    { eapply Proper_cmd; [reflexivity..|eassumption| |eapply Hpc].
+      intros tj mj lj (vj&dP&?&dQ); eauto 9. }
+    { eapply Hpost, Qi, Hpc. }
+  Qed.
+
+  Lemma tailrec2
+    e c t (m : mem) l (post : _->_->_-> Prop)
+    {measure : Type} {X} (P Q:_->X->_->_->_->Prop) lt (Hwf : well_founded lt)
+    (v0 : measure) (x0 : X)
+    (Hpre : P v0 x0 t m l)
+    (Hbody : forall v x t m l, P v x t m l ->
+      exists br, expr m l e (eq br) /\
+      (word_test br = true -> cmd rely guarantee progress call c t m l
+        (fun t' m' l' => exists v' x', P v' x' t' m' l' /\
+          (progress t' t \/ lt v' v) /\
+          forall T M L, Q v' x' T M L -> Q v x T M L)) /\
+      (word_test br = false -> Q v x t m l))
+    (Hpost : forall t m l, Q v0 x0 t m l -> post t m l)
+    : cmd rely guarantee progress call (cmd.while e c) t m l post.
+  Proof.
+    eexists measure, lt, (fun v t m l => exists x, P v x t m l /\
+                          forall T M L, Q v x T M L -> Q v0 x0 T M L).
+    split. assumption.
+    split; [solve[eauto]|].
+    intros vi ti mi li (?&?&Qi).
+    destruct (Hbody _ _ _ _ _ ltac:(eassumption)) as (br&?&XX); exists br; split; [assumption|].
+    destruct XX as (Htrue&Hfalse). split; intros Hbr;
+      [pose proof(Htrue Hbr)as Hpc|pose proof(Hfalse Hbr)as Hpc]; clear Hbr Htrue Hfalse.
+    { eapply Proper_cmd; [reflexivity..|eassumption| |eapply Hpc].
+      intros tj mj lj (vj&xj&dP&?&dQ); eauto 9. }
+    { eapply Hpost, Qi, Hpc. }
+  Qed.
+  Notation tailrec1 := tailrec.
+
+  Lemma tailrec3
+    e c t (m : mem) l (post : _->_->_-> Prop)
+    {measure : Type} {X Y} (P Q:_->X->Y->_->_->_->Prop) lt (Hwf : well_founded lt)
+    (v0 : measure) (x0 : X) (y0 : Y)
+    (Hpre : P v0 x0 y0 t m l)
+    (Hbody : forall v x y t m l, P v x y t m l ->
+      exists br, expr m l e (eq br) /\
+      (word_test br = true -> cmd rely guarantee progress call c t m l
+        (fun t' m' l' => exists v' x' y', P v' x' y' t' m' l' /\
+          (progress t' t \/ lt v' v) /\
+          forall T M L, Q v' x' y' T M L -> Q v x y T M L)) /\
+      (word_test br = false -> Q v x y t m l))
+    (Hpost : forall t m l, Q v0 x0 y0 t m l -> post t m l)
+    : cmd rely guarantee progress call (cmd.while e c) t m l post.
+  Proof.
+    eexists measure, lt, (fun v t m l => exists x y, P v x y t m l /\
+                          forall T M L, Q v x y T M L -> Q v0 x0 y0 T M L).
+    split. assumption.
+    split; [solve[eauto]|].
+    intros vi ti mi li (?&?&?&Qi).
+    destruct (Hbody _ _ _ _ _ _ ltac:(eassumption)) as (br&?&XX); exists br; split; [assumption|].
+    destruct XX as (Htrue&Hfalse). split; intros Hbr;
+      [pose proof(Htrue Hbr)as Hpc|pose proof(Hfalse Hbr)as Hpc]; clear Hbr Htrue Hfalse.
+    { eapply Proper_cmd; [reflexivity..|eassumption| |eapply Hpc].
+      intros tj mj lj (vj&xj&yj&dP&?&dQ); eauto 9. }
+    { eapply Hpost, Qi, Hpc. }
+  Qed.
+
+  Context {mem_ok : map.ok mem}.
+  Local Infix "*" := Separation.sep.
+  Local Infix "*" := Separation.sep : type_scope.
+  Local Infix "==>" := Lift1Prop.impl1.
+
+  Lemma tailrec_sep
     e c t (m : mem) l (post : _->_->_-> Prop)
     {measure : Type} P Q lt (Hwf : well_founded lt) (v0 : measure) R0
     (Hpre : (P v0 t l * R0) m)
